shift-reset/interpreter/builtin.v
@@ -1,27 +1,84 @@
 From Stdlib Require Import List String ZArith.
 From shift_reset.lib Require list.
 From shift_reset.lib Require Import int.
-From shift_reset.core Require Import syntax tag.
-From shift_reset.interpreter Require Import ierror imonad unwrap.
+From shift_reset.core Require Import syntax loc tag.
+From shift_reset.interpreter Require Import ierror iheap imonad unwrap.
 Import ListNotations.
 
 Local Open Scope string_scope.
 Local Open Scope imonad_scope.
 
 Definition string_length (v : val) : imonad val :=
-  s <- unwrap_vstring v;
-  imonad_pure (VInt (Z.of_nat (String.length s))).
+  let+ s := unwrap_vstring v in VInt (Z.of_nat (String.length s)).
+
+Definition array_length (v : val) : imonad val :=
+  let+ '(Array _ z) := unwrap_varray v in VInt z.
+
+Fixpoint array_free_loop (n : nat) (l : loc) (h : iheap) : option iheap :=
+  match n with
+  | O => Some h
+  | S n' =>
+      match iheap_dealloc l h with
+      | Some h' => array_free_loop n' (loc_succ l) h'
+      | None => None
+      end
+  end.
+
+Definition array_free (v : val) : imonad val :=
+  let* '(Array l z) := unwrap_varray v in
+  let* h := imonad_get_heap in
+  match array_free_loop (Z.to_nat z) l h with
+  | Some h' => VTt <$ imonad_set_heap h'
+  | None => imonad_throw_error (Memory_error "array_free")
+  end.
+
+Definition ref_free (v : val) : imonad val :=
+  let* l := unwrap_vref v in
+  let* h := imonad_get_heap in
+  match iheap_dealloc l h with
+  | Some h' => VTt <$ imonad_set_heap h'
+  | None => imonad_throw_error (Memory_error "ref_free")
+  end.
 
 Definition int_to_string (v : val) : imonad val :=
-  z <- unwrap_vint v;
-  imonad_pure (VString (Z_to_string z)).
+  let+ z := unwrap_vint v in VString (Z_to_string z).
 
-Definition builtin_registry : list (tag * (val -> imonad val)) :=
-  [(Tag "string_length", string_length);
-   (Tag "int_to_string", int_to_string)].
+Definition builtin1_registry : list (tag * (val -> imonad val)) :=
+  [(Tag "int_to_string", int_to_string);
+   (Tag "string_length", string_length);
+   (Tag "array_length", array_length);
+   (Tag "ref_free", ref_free);
+   (Tag "array_free", array_free)].
 
-Definition dispatch_builtin (tag : tag) : imonad (val -> imonad val) :=
-  match list.lookup tag_eqb tag builtin_registry with
+Definition dispatch_builtin1 (tag : tag) : imonad (val -> imonad val) :=
+  match list.lookup tag_eqb tag builtin1_registry with
+  | Some f => imonad_pure f
+  | None => imonad_throw_error (Name_error (tag_car tag))
+  end.
+
+Fixpoint array_make_loop (n : nat) (v : val) (h : iheap) : option iheap :=
+  match n with
+  | O => Some h
+  | S n' =>
+      match iheap_alloc v h with
+      | Some (_, h') => array_make_loop n' v h'
+      | None => None
+      end
+  end.
+
+Definition array_make (v1 v2 : val) : imonad val :=
+  let* z := unwrap_vint v1 in
+  let* h := imonad_get_heap in
+  match array_make_loop (Z.to_nat z) v2 h with
+  | Some h' => VArray (iheap_next_loc h) z <$ imonad_set_heap h'
+  | None => imonad_throw_error (Memory_error "array_make")
+  end.
+
+Definition builtin2_registry : list (tag * (val -> val -> imonad val)) :=
+  [(Tag "array_make", array_make)].
+
+Definition dispatch_builtin2 (tag : tag) : imonad (val -> val -> imonad val) :=
+  match list.lookup tag_eqb tag builtin2_registry with
   | Some f => imonad_pure f
   | None => imonad_throw_error (Name_error (tag_car tag))
   end.
