shift-reset/interpreter/iheap.v
@@ -1,19 +1,27 @@
-From shift_reset.lib Require option.
-From shift_reset.core Require Import syntax heap loc.
+From shift_reset.core Require Import syntax loc.
 
-Record iheap : Type := IHeap { iheap_car : heap; iheap_next_loc : loc }.
+Record iheap : Type := IHeap { iheap_car : LocMap.t val; iheap_next_loc : loc }.
 
 Definition iheap_empty : iheap :=
-  IHeap heap_empty loc_init.
+  IHeap LocMap.empty loc_init.
 
-Definition iheap_ref (v : val) (h : iheap) : option (loc * iheap) :=
-  let (h, l) := h in option.map (fun h' => (l, IHeap h' (loc_succ l))) (heap_ref l v h).
+Definition iheap_alloc (v : val) (h : iheap) : option (loc * iheap) :=
+  let (m, l) := h in
+  if LocMap.member l m
+  then None
+  else Some (l, IHeap (LocMap.insert l v m) (loc_succ l)).
 
-Definition iheap_get (l : loc) (h : iheap) : option val :=
-  heap_get l (iheap_car h).
+Definition iheap_read (l : loc) (h : iheap) : option val :=
+  LocMap.lookup l (iheap_car h).
 
-Definition iheap_set (l : loc) (v : val) (h : iheap) : option iheap :=
-  let (h, l') := h in option.map (fun h' => IHeap h' l') (heap_set l v h).
+Definition iheap_write (l : loc) (v : val) (h : iheap) : option iheap :=
+  let (m, l') := h in
+  if LocMap.member l m
+  then Some (IHeap (LocMap.insert l v m) l')
+  else None.
 
-Definition iheap_free (l : loc) (h : iheap) : option iheap :=
-  let (h, l') := h in option.map (fun h' => IHeap h' l') (heap_free l h).
+Definition iheap_dealloc (l : loc) (h : iheap) : option iheap :=
+  let (m, l') := h in
+  if LocMap.member l m
+  then Some (IHeap (LocMap.remove l m) l')
+  else None.
