shift-reset/interpreter/imonad.v
@@ -163,9 +163,11 @@ Notation "m1 <*> m2" := (imonad_app m1 m2) (at level 55, left associativity) : i
 Notation "m >>= f" := (imonad_bind m f) (at level 50, left associativity) : imonad_scope.
 Notation "m1 >> m2" := (imonad_then m1 m2) (at level 50, left associativity) : imonad_scope.
 
-Notation "' x <- m1 ; m2" := (imonad_bind m1 (fun x => m2)) (at level 100, x pattern, right associativity) : imonad_scope.
-Notation "x <- m1 ; m2" := (imonad_bind m1 (fun x => m2)) (at level 100, right associativity) : imonad_scope.
-Notation "m1 ;; m2" := (imonad_bind m1 (fun _ => m2)) (at level 100, right associativity) : imonad_scope.
+Notation "let+ x := m 'in' y" :=
+  (imonad_map (fun x => y) m) (at level 100, x binder, right associativity) : imonad_scope.
+
+Notation "let* x := m1 'in' m2" :=
+  (imonad_bind m1 (fun x => m2)) (at level 100, x binder, right associativity) : imonad_scope.
 
 Definition imonad_kleisli_compose {A B C} (f1 : A -> imonad B) (f2 : B -> imonad C) (x : A) : imonad C :=
   f1 x >>= f2.
@@ -174,7 +176,7 @@ Fixpoint imonad_list_map {A B} (f : A -> imonad B) (xs : list A) : imonad (list 
   match xs with
   | [] => imonad_pure []
   | x :: xs' =>
-      y <- f x;
+      let* y := f x in
       cons y <$> imonad_list_map f xs'
   end.
 
@@ -182,7 +184,7 @@ Fixpoint imonad_list_forall2b {A B} (f : A -> B -> imonad bool) (xs : list A) (y
   match xs, ys with
   | [], [] => imonad_pure true
   | x :: xs', y :: ys' =>
-      b <- f x y;
+      let* b := f x y in
       if b then imonad_list_forall2b f xs' ys' else imonad_pure false
   | _, _ => imonad_pure false
   end.
