shift-reset/interpreter/interpreter.v
@@ -4,12 +4,31 @@ From shift_reset.interpreter Require Import builtin ierror iheap imonad op unwra
 
 Local Open Scope string_scope.
 Local Open Scope imonad_scope.
+Local Open Scope Z_scope.
 Local Unset Elimination Schemes.
+
+Definition dispatch_get_at (v1 v2 : val) : imonad val :=
+  match v1, v2 with
+  | VString s, VInt i =>
+      match String.get (Z.to_nat i) s with
+      | None => imonad_throw_error (Invalid_argument "index out of bounds")
+      | Some a => imonad_pure (VChar a)
+      end
+  | VArray l z, VInt i =>
+      if i <? z then
+        let* h := imonad_get_heap in
+        match iheap_read (loc_add l (Z.to_N i)) h with
+        | None => imonad_throw_error (Memory_error "array_get_at")
+        | Some v => imonad_pure v
+        end
+      else imonad_throw_error (Invalid_argument "index out of bounds")
+  | _, _ => imonad_throw_error (Type_error "dispatch_get_at")
+  end.
 
 Fixpoint interpret_val_term (t : val_term) : imonad val :=
   match t with
   | TVVar x =>
-      e <- imonad_ask_env;
+      let* e := imonad_ask_env in
       match env_lookup x e with
       | None => imonad_throw_error (Name_error (var_car x))
       | Some v => imonad_pure v
@@ -22,30 +41,30 @@ Fixpoint interpret_val_term (t : val_term) : imonad val :=
   | TVChar a => imonad_pure (VChar a)
   | TVString s => imonad_pure (VString s)
   | TVAnd t1 t2 =>
-      v <- interpret_val_term t1;
-      b <- unwrap_vbool v;
+      let* v := interpret_val_term t1 in
+      let* b := unwrap_vbool v in
       if b then interpret_val_term t2 else imonad_pure VFalse
   | TVOr t1 t2 =>
-      v <- interpret_val_term t1;
-      b <- unwrap_vbool v;
+      let* v := interpret_val_term t1 in
+      let* b := unwrap_vbool v in
       if b then imonad_pure VTrue else interpret_val_term t2
   | TVFun b t' => imonad_asks_env (VFun b t')
   | TVFix f b t' => imonad_asks_env (VFix f b t')
   | TVFixMut t' f => imonad_asks_env (VFixMut t' f)
   | TVPair t1 t2 =>
-      v <- interpret_val_term t1;
+      let* v := interpret_val_term t1 in
       VPair v <$> interpret_val_term t2
   | TVFst t' =>
-      v <- interpret_val_term t';
+      let* v := interpret_val_term t' in
       fst <$> unwrap_vprod v
   | TVSnd t' =>
-      v <- interpret_val_term t';
+      let* v := interpret_val_term t' in
       snd <$> unwrap_vprod v
   | TVTuple t' => VTuple <$> interpret_tuple_term t'
   | TVRecord t' => VRecord <$> interpret_record_term t'
   | TVProj t' tag =>
-      v <- interpret_val_term t';
-      r <- unwrap_vrecord v;
+      let* v := interpret_val_term t' in
+      let* r := unwrap_vrecord v in
       match record_lookup tag r with
       | None => imonad_throw_error (Name_error (tag_car tag))
       | Some v' => imonad_pure v'
@@ -54,73 +73,75 @@ Fixpoint interpret_val_term (t : val_term) : imonad val :=
   | TVInr t' => VInr <$> interpret_val_term t'
   | TVVariant tag t' => VVariant tag <$> interpret_val_term t'
   | TVRef t' =>
-      v <- interpret_val_term t';
-      h <- imonad_get_heap;
-      match iheap_ref v h with
-      | None => imonad_throw_error (Memory_error "ref")
+      let* v := interpret_val_term t' in
+      let* h := imonad_get_heap in
+      match iheap_alloc v h with
+      | None => imonad_throw_error (Memory_error "new_ref")
       | Some (l, h') => VRef l <$ imonad_set_heap h'
       end
   | TVGet t' =>
-      v <- interpret_val_term t';
-      l <- unwrap_vref v;
-      h <- imonad_get_heap;
-      match iheap_get l h with
-      | None => imonad_throw_error (Memory_error "get")
+      let* v := interpret_val_term t' in
+      let* l := unwrap_vref v in
+      let* h := imonad_get_heap in
+      match iheap_read l h with
+      | None => imonad_throw_error (Memory_error "ref_get")
       | Some v' => imonad_pure v'
       end
   | TVSet t1 t2 =>
-      v <- interpret_val_term t1;
-      l <- unwrap_vref v;
-      v <- interpret_val_term t2;
-      h <- imonad_get_heap;
-      match iheap_set l v h with
-      | None => imonad_throw_error (Memory_error "set")
+      let* v1 := interpret_val_term t1 in
+      let* v2 := interpret_val_term t2 in
+      let* l := unwrap_vref v1 in
+      let* h := imonad_get_heap in
+      match iheap_write l v2 h with
+      | None => imonad_throw_error (Memory_error "ref_set")
       | Some h' => VTt <$ imonad_set_heap h'
       end
   | TVGetAt t1 t2 =>
-      v <- interpret_val_term t1;
-      s <- unwrap_vstring v;
-      v <- interpret_val_term t2;
-      z <- unwrap_vint v;
-      match String.get (Z.to_nat z) s with
-      | None => imonad_throw_error (Invalid_argument "index out of bounds")
-      | Some a => imonad_pure (VChar a)
-      end
-  | TVFree t' =>
-      v <- interpret_val_term t';
-      l <- unwrap_vref v;
-      h <- imonad_get_heap;
-      match iheap_free l h with
-      | None => imonad_throw_error (Memory_error "free")
-      | Some h' => VTt <$ imonad_set_heap h'
-      end
+      let* v := interpret_val_term t1 in
+      interpret_val_term t2 >>= dispatch_get_at v
+  | TVSetAt t1 t2 t3 =>
+      let* v1 := interpret_val_term t1 in
+      let* v2 := interpret_val_term t2 in
+      let* v3 := interpret_val_term t3 in
+      let* '(Array l z) := unwrap_varray v1 in
+      let* i := unwrap_vint v2 in
+      if i <? z then
+        let* h := imonad_get_heap in
+        match iheap_write (loc_add l (Z.to_N i)) v3 h with
+        | None => imonad_throw_error (Memory_error "array_set_at")
+        | Some h' => VTt <$ imonad_set_heap h'
+        end
+      else imonad_throw_error (Invalid_argument "index out of bounds")
   | TVExn tag t' => VExn tag <$> interpret_val_term t'
   | TVEff tag t' => VEff tag <$> interpret_val_term t'
   | TVAssert t' =>
-      v <- interpret_val_term t';
-      b <- unwrap_vbool v;
+      let* v := interpret_val_term t' in
+      let* b := unwrap_vbool v in
       if b then imonad_pure VTt else imonad_throw_error (Assert_failure "")
   | TVOp1 op t' => interpret_val_term t' >>= dispatch_op1 op
   | TVOp2 op t1 t2 =>
-      v <- interpret_val_term t1;
-      f <- dispatch_op2 op v;
-      interpret_val_term t2 >>= f
-  | TVBuiltin tag t' =>
-      f <- dispatch_builtin tag;
+      let* v := interpret_val_term t1 in
+      interpret_val_term t2 >>= dispatch_op2 op v
+  | TVBuiltin1 tag t' =>
+      let* f := dispatch_builtin1 tag in
       interpret_val_term t' >>= f
+  | TVBuiltin2 tag t1 t2 =>
+      let* f := dispatch_builtin2 tag in
+      let* v := interpret_val_term t1 in
+      interpret_val_term t2 >>= f v
   end
 with interpret_tuple_term (t : tuple_term) : imonad tuple :=
   match t with
   | TTupleNil => imonad_pure TupleNil
   | TTupleCons t1 t2 =>
-      v <- interpret_val_term t1;
+      let* v := interpret_val_term t1 in
       TupleCons v <$> interpret_tuple_term t2
   end
 with interpret_record_term (t : record_term) : imonad record :=
   match t with
   | TRecordNil => imonad_pure RecordNil
   | TRecordCons tag t1 t2 =>
-      v <- interpret_val_term t1;
+      let* v := interpret_val_term t1 in
       RecordCons tag v <$> interpret_record_term t2
   end.
 
@@ -195,12 +216,6 @@ Inductive iresult : Type :=
 | IRControl : metakont -> (val -> imonad iresult) -> iresult
 | IRRaise : tag -> val -> iresult
 | IRPerform : metakont -> tag -> val -> iresult.
-
-Definition IRPerform' (mk : metakont) (e : eff) : iresult :=
-  let (tag, v) := e in IRPerform mk tag v.
-
-Definition IRRaise' (e : exn) : iresult :=
-  let (tag, v) := e in IRRaise tag v.
 
 Record ikont : Type := IKont { ikont_car :> kont; ikont_app : val -> imonad iresult }.
 
@@ -368,89 +383,91 @@ Definition interpret_term (self : interpreter) : term -> ikont -> imonad iresult
     match t with
     | TVal tv => interpret_val_term tv >>= ikont_app k
     | TApp t1 t2 =>
-        u <- interpret_val_term t1;
-        c <- unwrap_vclosure u;
-        v <- interpret_val_term t2;
+        let* v1 := interpret_val_term t1 in
+        let* v2 := interpret_val_term t2 in
+        let* c := unwrap_vclosure v1 in
         match c with
-        | CFun b t' e => imonad_under_env (with_binder b v e) (self t' k)
-        | CFix f b t' e => imonad_under_env (with_binder b v (ECons f u e)) (self t' k)
-        | CFixMut t' f e => interpret_fix_mut_term_under (with_fix_mut_term t' e) self t' k f v
-        | CMKPure mk => interpret_metakont_app self mk k v
-        | CMKReset mk => interpret_metakont self mk v >>= unwind_reset k
-        | CMKHandle mk t1' t2' e => interpret_metakont self mk v >>= unwind_handle e self t1' t2' k
+        | CFun b t' e => imonad_under_env (with_binder b v2 e) (self t' k)
+        | CFix f b t' e => imonad_under_env (with_binder b v2 (ECons f v1 e)) (self t' k)
+        | CFixMut t' f e => interpret_fix_mut_term_under (with_fix_mut_term t' e) self t' k f v2
+        | CMKPure mk => interpret_metakont_app self mk k v2
+        | CMKReset mk => interpret_metakont self mk v2 >>= unwind_reset k
+        | CMKHandle mk t1' t2' e => interpret_metakont self mk v2 >>= unwind_handle e self t1' t2' k
         end
     | TSeq t1 t2 =>
-        e <- imonad_ask_env;
+        let* e := imonad_ask_env in
         self' t1 (IKont (KSeq t2 e k) (fun _ => imonad_under_env e (self' t2 k)))
     | TLet b t1 t2 =>
-        e <- imonad_ask_env;
+        let* e := imonad_ask_env in
         self' t1 (IKont (KLet b t2 e k) (fun v => imonad_under_env (with_binder b v e) (self' t2 k)))
     | TIf tv t1 t2 =>
-        v <- interpret_val_term tv;
-        b <- unwrap_vbool v;
+        let* v := interpret_val_term tv in
+        let* b := unwrap_vbool v in
         if b then self' t1 k else self' t2 k
     | TSplit b1 b2 tv t' =>
-        v <- interpret_val_term tv;
-        '(v1, v2) <- unwrap_vprod v;
+        let* v := interpret_val_term tv in
+        let* '(v1, v2) := unwrap_vprod v in
         imonad_local_env (fun e => with_binder b2 v2 (with_binder b1 v1 e)) (self' t' k)
     | TCase tv b1 t1 b2 t2 =>
-        v <- interpret_val_term tv;
-        s <- unwrap_vsum v;
+        let* v := interpret_val_term tv in
+        let* s := unwrap_vsum v in
         match s with
         | inl v' => imonad_local_env (with_binder b1 v') (self' t1 k)
         | inr v' => imonad_local_env (with_binder b2 v') (self' t2 k)
         end
     | TWhile tv t' =>
-        v <- interpret_val_term tv;
-        b <- unwrap_vbool v;
+        let* v := interpret_val_term tv in
+        let* b := unwrap_vbool v in
         if b then
-          e <- imonad_ask_env;
+          let* e := imonad_ask_env in
           self' t' (IKont (KSeq t e k) (fun _ => imonad_under_env e (self t k)))
         else ikont_app k VTt
     | TLetFix f b t1 t2 => imonad_local_env (fun e => ECons f (VFix f b t1 e) e) (self' t2 k)
     | TLetFixMut t1 t2 => imonad_local_env (with_fix_mut_term t1) (self' t2 k)
     | TLetTuple p tv t' =>
-        v <- interpret_val_term tv;
-        t <- unwrap_vtuple v;
-        e <- imonad_ask_env;
+        let* v := interpret_val_term tv in
+        let* t := unwrap_vtuple v in
+        let* e := imonad_ask_env in
         match match_tuple p t e with
         | Some e' => imonad_under_env e' (self' t' k)
         | None => imonad_throw_error (Match_failure "")
         end
     | TLetRecord p tv t' =>
-        v <- interpret_val_term tv;
-        r <- unwrap_vrecord v;
-        e <- imonad_ask_env;
+        let* v := interpret_val_term tv in
+        let* r := unwrap_vrecord v in
+        let* e := imonad_ask_env in
         match match_record p r e with
         | Some e' => imonad_under_env e' (self' t' k)
         | None => imonad_throw_error (Match_failure "")
         end
     | TMatchVariant tv t' =>
-        v <- interpret_val_term tv;
-        '(Variant tag v') <- unwrap_vvariant v;
-        e <- imonad_ask_env;
+        let* v := interpret_val_term tv in
+        let* '(Variant tag v') := unwrap_vvariant v in
+        let* e := imonad_ask_env in
         interpret_variant_term_under e self' t' k tag v'
     | TShift b t' => imonad_asks_env (fun e => IRShift (MKPure k) (fun u => imonad_under_env (with_binder b u e) (self' t' ikont_nil)))
     | TReset t' => self' t' ikont_nil >>= unwind_reset k
     | TControl b t' => imonad_asks_env (fun e => IRControl (MKPure k) (fun u => imonad_under_env (with_binder b u e) (self' t' ikont_nil)))
     | TPrompt t' => self' t' ikont_nil >>= unwind_prompt k
     | TRaise t' =>
-        v <- interpret_val_term t';
-        IRRaise' <$> unwrap_vexn v
+        let* v := interpret_val_term t' in
+        let+ '(Exn tag v') := unwrap_vexn v in
+        IRRaise tag v'
     | TTry t1 t2 =>
-        r <- self' t1 ikont_nil;
-        e <- imonad_ask_env;
+        let* r := self' t1 ikont_nil in
+        let* e := imonad_ask_env in
         unwind_try e self' t2 k r
     | TPerform t' =>
-        v <- interpret_val_term t';
-        IRPerform' (MKPure k) <$> unwrap_veff v
+        let* v := interpret_val_term t' in
+        let+ '(Eff tag v') := unwrap_veff v in
+        IRPerform (MKPure k) tag v'
     | THandle t1 t2 t3 =>
-        r <- self' t1 ikont_nil;
-        e <- imonad_ask_env;
+        let* r := self' t1 ikont_nil in
+        let* e := imonad_ask_env in
         unwind_handle e self' t2 t3 k r
     | TShallowHandle t1 t2 t3 =>
-        r <- self' t1 ikont_nil;
-        e <- imonad_ask_env;
+        let* r := self' t1 ikont_nil in
+        let* e := imonad_ask_env in
         unwind_shallow_handle e self' t2 t3 k r
     end.
 
