shift-reset/interpreter/op.v
@@ -1,10 +1,13 @@
-From Stdlib Require Import Ascii String Qcanon ZArith.
-From shift_reset.lib Require Import char comparison float int string.
+From Stdlib Require Import Ascii Bool String Qcanon ZArith.
+From shift_reset.lib Require Import comparison.
 From shift_reset.core Require Import syntax loc tag val.
 From shift_reset.interpreter Require Import ierror imonad unwrap.
 
 Local Open Scope string_scope.
 Local Open Scope imonad_scope.
+Local Open Scope lazy_bool_scope.
+
+(** Op1 *)
 
 Definition dispatch_pos (v : val) : imonad val :=
   match v with
@@ -34,74 +37,46 @@ Definition dispatch_op1 (op : op1) : val -> imonad val :=
   | Op1Not => dispatch_not
   end.
 
-Definition vint_add (z : Z) (arg : val) : imonad val :=
-  VInt_by2 Z.add z <$> unwrap_vint arg.
+(** Op2 *)
 
-Definition vint_sub (z : Z) (arg : val) : imonad val :=
-  VInt_by2 Z.sub z <$> unwrap_vint arg.
-
-Definition vint_mul (z : Z) (arg : val) : imonad val :=
-  VInt_by2 Z.mul z <$> unwrap_vint arg.
-
-Definition vint_div (z : Z) (arg : val) : imonad val :=
-  VInt_by2 Z.div z <$> unwrap_vint arg.
-
-Definition vint_mod (z : Z) (arg : val) : imonad val :=
-  VInt_by2 Z.modulo z <$> unwrap_vint arg.
-
-Definition vfloat_add (q : Qc) (arg : val) : imonad val :=
-  VFloat_by2 Qcplus q <$> unwrap_vfloat arg.
-
-Definition vfloat_sub (q : Qc) (arg : val) : imonad val :=
-  VFloat_by2 Qcminus q <$> unwrap_vfloat arg.
-
-Definition vfloat_mul (q : Qc) (arg : val) : imonad val :=
-  VFloat_by2 Qcmult q <$> unwrap_vfloat arg.
-
-Definition vfloat_div (q : Qc) (arg : val) : imonad val :=
-  VFloat_by2 Qcdiv q <$> unwrap_vfloat arg.
-
-Definition vstring_app (s : string) (arg : val) : imonad val :=
-  VString_by2 String.append s <$> unwrap_vstring arg.
-
-Definition dispatch_add (v : val) : imonad (val -> imonad val) :=
-  match v with
-  | VInt z => imonad_pure (vint_add z)
-  | VFloat q => imonad_pure (vfloat_add q)
-  | _ => imonad_throw_error (Type_error "dispatch_add")
+Definition dispatch_add (v1 v2 : val) : imonad val :=
+  match v1, v2 with
+  | VInt z1, VInt z2 => imonad_pure (VInt (Z.add z1 z2))
+  | VFloat q1, VFloat q2 => imonad_pure (VFloat (Qcplus q1 q2))
+  | _, _ => imonad_throw_error (Type_error "dispatch_add")
   end.
 
-Definition dispatch_sub (v : val) : imonad (val -> imonad val) :=
-  match v with
-  | VInt z => imonad_pure (vint_sub z)
-  | VFloat q => imonad_pure (vfloat_sub q)
-  | _ => imonad_throw_error (Type_error "dispatch_sub")
+Definition dispatch_sub (v1 v2 : val) : imonad val :=
+  match v1, v2 with
+  | VInt z1, VInt z2 => imonad_pure (VInt (Z.sub z1 z2))
+  | VFloat q1, VFloat q2 => imonad_pure (VFloat (Qcminus q1 q2))
+  | _, _ => imonad_throw_error (Type_error "dispatch_sub")
   end.
 
-Definition dispatch_mul (v : val) : imonad (val -> imonad val) :=
-  match v with
-  | VInt z => imonad_pure (vint_mul z)
-  | VFloat q => imonad_pure (vfloat_mul q)
-  | _ => imonad_throw_error (Type_error "dispatch_mul")
+Definition dispatch_mul (v1 v2 : val) : imonad val :=
+  match v1, v2 with
+  | VInt z1, VInt z2 => imonad_pure (VInt (Z.mul z1 z2))
+  | VFloat q1, VFloat q2 => imonad_pure (VFloat (Qcmult q1 q2))
+  | _, _ => imonad_throw_error (Type_error "dispatch_mul")
   end.
 
-Definition dispatch_div (v : val) : imonad (val -> imonad val) :=
-  match v with
-  | VInt z => imonad_pure (vint_div z)
-  | VFloat q => imonad_pure (vfloat_div q)
-  | _ => imonad_throw_error (Type_error "dispatch_div")
+Definition dispatch_div (v1 v2 : val) : imonad val :=
+  match v1, v2 with
+  | VInt z1, VInt z2 => imonad_pure (VInt (Z.div z1 z2))
+  | VFloat q1, VFloat q2 => imonad_pure (VFloat (Qcdiv q1 q2))
+  | _, _ => imonad_throw_error (Type_error "dispatch_div")
   end.
 
-Definition dispatch_mod (v : val) : imonad (val -> imonad val) :=
-  match v with
-  | VInt z => imonad_pure (vint_mod z)
-  | _ => imonad_throw_error (Type_error "dispatch_mod")
+Definition dispatch_mod (v1 v2 : val) : imonad val :=
+  match v1, v2 with
+  | VInt z1, VInt z2 => imonad_pure (VInt (Z.modulo z1 z2))
+  | _, _ => imonad_throw_error (Type_error "dispatch_mod")
   end.
 
-Definition dispatch_app (v : val) : imonad (val -> imonad val) :=
-  match v with
-  | VString s => imonad_pure (vstring_app s)
-  | _ => imonad_throw_error (Type_error "dispatch_app")
+Definition dispatch_app (v1 v2 : val) : imonad val :=
+  match v1, v2 with
+  | VString s1, VString s2 => imonad_pure (VString (String.append s1 s2))
+  | _, _ => imonad_throw_error (Type_error "dispatch_app")
   end.
 
 Fixpoint compare_val (v1 v2 : val) : imonad comparison :=
@@ -116,7 +91,7 @@ Fixpoint compare_val (v1 v2 : val) : imonad comparison :=
   | VChar a1, VChar a2 => imonad_pure (Ascii.compare a1 a2)
   | VString s1, VString s2 => imonad_pure (String.compare s1 s2)
   | VPair v11 v12, VPair v21 v22 =>
-      c <- compare_val v11 v21;
+      let* c := compare_val v11 v21 in
       match c with
       | Eq => compare_val v12 v22
       | _ => imonad_pure c
@@ -126,28 +101,6 @@ Fixpoint compare_val (v1 v2 : val) : imonad comparison :=
   | VInl _, VInr _ => imonad_pure Lt
   | VInr _, VInl _ => imonad_pure Gt
   | _, _ => imonad_throw_error (Type_error "compare_val")
-  end.
-
-Definition vprod_compare (v1 v2 arg : val) : imonad comparison :=
-  '(v1', v2') <- unwrap_vprod arg;
-  c <- compare_val v1 v1';
-  match c with
-  | Eq => compare_val v2 v2'
-  | _ => imonad_pure c
-  end.
-
-Definition vsum_compare1 (v arg : val) : imonad comparison :=
-  s <- unwrap_vsum arg;
-  match s with
-  | inl v' => compare_val v v'
-  | inr _ => imonad_pure Lt
-  end.
-
-Definition vsum_compare2 (v arg : val) : imonad comparison :=
-  s <- unwrap_vsum arg;
-  match s with
-  | inl _ => imonad_pure Gt
-  | inr v' => compare_val v v'
   end.
 
 Fixpoint equal_val (v1 v2 : val) : imonad bool :=
@@ -162,7 +115,7 @@ Fixpoint equal_val (v1 v2 : val) : imonad bool :=
   | VChar a1, VChar a2 => imonad_pure (Ascii.eqb a1 a2)
   | VString s1, VString s2 => imonad_pure (String.eqb s1 s2)
   | VPair v11 v12, VPair v21 v22 =>
-      b <- equal_val v11 v21;
+      let* b := equal_val v11 v21 in
       if b then equal_val v12 v22 else imonad_pure false
   | VTuple t1, VTuple t2 => equal_tuple t1 t2
   | VRecord r1, VRecord r2 => equal_record r1 r2
@@ -174,13 +127,14 @@ Fixpoint equal_val (v1 v2 : val) : imonad bool :=
   | VRef l1, VRef l2 => imonad_pure (loc_eqb l1 l2)
   | VExn tag1 v1', VExn tag2 v2' => if tag_eqb tag1 tag2 then equal_val v1' v2' else imonad_pure false
   | VEff tag1 v1', VEff tag2 v2' => if tag_eqb tag1 tag2 then equal_val v1' v2' else imonad_pure false
+  | VArray l1 z1, VArray l2 z2 => imonad_pure (loc_eqb l1 l2 &&& Z.eqb z1 z2)
   | _, _ => imonad_throw_error (Type_error "equal_val")
   end
 with equal_tuple (t1 t2 : tuple) : imonad bool :=
   match t1, t2 with
   | TupleNil, TupleNil => imonad_pure true
   | TupleCons v1 t1', TupleCons v2 t2' =>
-      b <- equal_val v1 v2;
+      let* b := equal_val v1 v2 in
       if b then equal_tuple t1' t2' else imonad_pure false
   | _, _ => imonad_pure false
   end
@@ -189,396 +143,31 @@ with equal_record (r1 r2 : record) : imonad bool :=
   | RecordNil, RecordNil => imonad_pure true
   | RecordCons tag1 v1 r1', RecordCons tag2 v2 r2' =>
       if tag_eqb tag1 tag2 then
-        b <- equal_val v1 v2;
+        let* b := equal_val v1 v2 in
         if b then equal_record r1' r2' else imonad_pure false
       else imonad_pure false
   | _, _ => imonad_pure false
   end.
 
-Definition vprod_equal (v1 v2 arg : val) : imonad bool :=
-  '(v1', v2') <- unwrap_vprod arg;
-  b <- equal_val v1 v1';
-  if b then equal_val v2 v2' else imonad_pure false.
+Definition dispatch_lt (v1 v2 : val) : imonad val :=
+  let+ c := compare_val v1 v2 in VBool (compare_ltb c).
 
-Definition vtuple_equal (t : tuple) (arg : val) : imonad bool :=
-  unwrap_vtuple arg >>= equal_tuple t.
+Definition dispatch_le (v1 v2 : val) : imonad val :=
+  let+ c := compare_val v1 v2 in VBool (compare_leb c).
 
-Definition vrecord_equal (r : record) (arg : val) : imonad bool :=
-  unwrap_vrecord arg >>= equal_record r.
+Definition dispatch_gt (v1 v2 : val) : imonad val :=
+  let+ c := compare_val v1 v2 in VBool (compare_gtb c).
 
-Definition vsum_equal1 (v arg : val) : imonad bool :=
-  s <- unwrap_vsum arg;
-  match s with
-  | inl v' => equal_val v v'
-  | inr _ => imonad_pure false
-  end.
+Definition dispatch_ge (v1 v2 : val) : imonad val :=
+  let+ c := compare_val v1 v2 in VBool (compare_geb c).
 
-Definition vsum_equal2 (v arg : val) : imonad bool :=
-  s <- unwrap_vsum arg;
-  match s with
-  | inl _ => imonad_pure false
-  | inr v' => equal_val v v'
-  end.
+Definition dispatch_eq (v1 v2 : val) : imonad val :=
+  VBool <$> equal_val v1 v2.
 
-Definition vvariant_equal (tag : tag) (v arg : val) : imonad bool :=
-  '(Variant tag' v') <- unwrap_vvariant arg;
-  if tag_eqb tag tag' then equal_val v v' else imonad_pure false.
+Definition dispatch_neq (v1 v2 : val) : imonad val :=
+  let+ b := equal_val v1 v2 in VBool (negb b).
 
-Definition vexn_equal (tag : tag) (v arg : val) : imonad bool :=
-  '(Exn tag' v') <- unwrap_vexn arg;
-  if tag_eqb tag tag' then equal_val v v' else imonad_pure false.
-
-Definition veff_equal (tag : tag) (v arg : val) : imonad bool :=
-  '(Eff tag' v') <- unwrap_veff arg;
-  if tag_eqb tag tag' then equal_val v v' else imonad_pure false.
-
-(** Unit *)
-
-Definition vunit_lt (arg : val) : imonad val :=
-  VFalse <$ unwrap_vunit arg.
-
-Definition vunit_le (arg : val) : imonad val :=
-  VTrue <$ unwrap_vunit arg.
-
-Definition vunit_gt (arg : val) : imonad val :=
-  VFalse <$ unwrap_vunit arg.
-
-Definition vunit_ge (arg : val) : imonad val :=
-  VTrue <$ unwrap_vunit arg.
-
-Definition vunit_eq (arg : val) : imonad val :=
-  VTrue <$ unwrap_vunit arg.
-
-Definition vunit_neq (arg : val) : imonad val :=
-  VFalse <$ unwrap_vunit arg.
-
-(** Int *)
-
-Definition vint_lt (z : Z) (arg : val) : imonad val :=
-  VBool_by2 Z.ltb z <$> unwrap_vint arg.
-
-Definition vint_le (z : Z) (arg : val) : imonad val :=
-  VBool_by2 Z.leb z <$> unwrap_vint arg.
-
-Definition vint_gt (z : Z) (arg : val) : imonad val :=
-  VBool_by2 Z.gtb z <$> unwrap_vint arg.
-
-Definition vint_ge (z : Z) (arg : val) : imonad val :=
-  VBool_by2 Z.geb z <$> unwrap_vint arg.
-
-Definition vint_eq (z : Z) (arg : val) : imonad val :=
-  VBool_by2 Z.eqb z <$> unwrap_vint arg.
-
-Definition vint_neq (z : Z) (arg : val) : imonad val :=
-  VBool_by2 Z_neqb z <$> unwrap_vint arg.
-
-(** Float *)
-
-Definition vfloat_lt (q : Qc) (arg : val) : imonad val :=
-  VBool_by2 Qc_ltb q <$> unwrap_vfloat arg.
-
-Definition vfloat_le (q : Qc) (arg : val) : imonad val :=
-  VBool_by2 Qc_leb q <$> unwrap_vfloat arg.
-
-Definition vfloat_gt (q : Qc) (arg : val) : imonad val :=
-  VBool_by2 Qc_gtb q <$> unwrap_vfloat arg.
-
-Definition vfloat_ge (q : Qc) (arg : val) : imonad val :=
-  VBool_by2 Qc_geb q <$> unwrap_vfloat arg.
-
-Definition vfloat_eq (q : Qc) (arg : val) : imonad val :=
-  VBool_by2 Qc_eq_bool q <$> unwrap_vfloat arg.
-
-Definition vfloat_neq (q : Qc) (arg : val) : imonad val :=
-  VBool_by2 Qc_neqb q <$> unwrap_vfloat arg.
-
-(** Bool *)
-
-Definition vbool_lt1 (arg : val) : imonad val :=
-  VFalse <$ unwrap_vbool arg.
-
-Definition vbool_le1 (arg : val) : imonad val :=
-  VBool <$> unwrap_vbool arg.
-
-Definition vbool_gt1 (arg : val) : imonad val :=
-  VBool_by negb <$> unwrap_vbool arg.
-
-Definition vbool_ge1 (arg : val) : imonad val :=
-  VTrue <$ unwrap_vbool arg.
-
-Definition vbool_eq1 (arg : val) : imonad val :=
-  VBool <$> unwrap_vbool arg.
-
-Definition vbool_neq1 (arg : val) : imonad val :=
-  VBool_by negb <$> unwrap_vbool arg.
-
-Definition vbool_lt2 (arg : val) : imonad val :=
-  VBool <$> unwrap_vbool arg.
-
-Definition vbool_le2 (arg : val) : imonad val :=
-  VTrue <$ unwrap_vbool arg.
-
-Definition vbool_gt2 (arg : val) : imonad val :=
-  VFalse <$ unwrap_vbool arg.
-
-Definition vbool_ge2 (arg : val) : imonad val :=
-  VBool_by negb <$> unwrap_vbool arg.
-
-Definition vbool_eq2 (arg : val) : imonad val :=
-  VBool_by negb <$> unwrap_vbool arg.
-
-Definition vbool_neq2 (arg : val) : imonad val :=
-  VBool <$> unwrap_vbool arg.
-
-(** Char *)
-
-Definition vchar_lt (a : ascii) (arg : val) : imonad val :=
-  VBool_by2 Ascii.ltb a <$> unwrap_vchar arg.
-
-Definition vchar_le (a : ascii) (arg : val) : imonad val :=
-  VBool_by2 Ascii.leb a <$> unwrap_vchar arg.
-
-Definition vchar_gt (a : ascii) (arg : val) : imonad val :=
-  VBool_by2 ascii_gtb a <$> unwrap_vchar arg.
-
-Definition vchar_ge (a : ascii) (arg : val) : imonad val :=
-  VBool_by2 ascii_geb a <$> unwrap_vchar arg.
-
-Definition vchar_eq (a : ascii) (arg : val) : imonad val :=
-  VBool_by2 Ascii.eqb a <$> unwrap_vchar arg.
-
-Definition vchar_neq (a : ascii) (arg : val) : imonad val :=
-  VBool_by2 ascii_neqb a <$> unwrap_vchar arg.
-
-(** String *)
-
-Definition vstring_lt (s : string) (arg : val) : imonad val :=
-  VBool_by2 String.ltb s <$> unwrap_vstring arg.
-
-Definition vstring_le (s : string) (arg : val) : imonad val :=
-  VBool_by2 String.leb s <$> unwrap_vstring arg.
-
-Definition vstring_gt (s : string) (arg : val) : imonad val :=
-  VBool_by2 string_gtb s <$> unwrap_vstring arg.
-
-Definition vstring_ge (s : string) (arg : val) : imonad val :=
-  VBool_by2 string_geb s <$> unwrap_vstring arg.
-
-Definition vstring_eq (s : string) (arg : val) : imonad val :=
-  VBool_by2 String.eqb s <$> unwrap_vstring arg.
-
-Definition vstring_neq (s : string) (arg : val) : imonad val :=
-  VBool_by2 string_neqb s <$> unwrap_vstring arg.
-
-(** Prod *)
-
-Definition vprod_lt (v1 v2 arg : val) : imonad val :=
-  VBool_by compare_ltb <$> vprod_compare v1 v2 arg.
-
-Definition vprod_le (v1 v2 arg : val) : imonad val :=
-  VBool_by compare_leb <$> vprod_compare v1 v2 arg.
-
-Definition vprod_gt (v1 v2 arg : val) : imonad val :=
-  VBool_by compare_gtb <$> vprod_compare v1 v2 arg.
-
-Definition vprod_ge (v1 v2 arg : val) : imonad val :=
-  VBool_by compare_geb <$> vprod_compare v1 v2 arg.
-
-Definition vprod_eq (v1 v2 arg : val) : imonad val :=
-  VBool <$> vprod_equal v1 v2 arg.
-
-Definition vprod_neq (v1 v2 arg : val) : imonad val :=
-  VBool_by negb <$> vprod_equal v1 v2 arg.
-
-(** Sum *)
-
-Definition vsum_lt1 (v arg : val) : imonad val :=
-  VBool_by compare_ltb <$> vsum_compare1 v arg.
-
-Definition vsum_le1 (v arg : val) : imonad val :=
-  VBool_by compare_leb <$> vsum_compare1 v arg.
-
-Definition vsum_gt1 (v arg : val) : imonad val :=
-  VBool_by compare_gtb <$> vsum_compare1 v arg.
-
-Definition vsum_ge1 (v arg : val) : imonad val :=
-  VBool_by compare_geb <$> vsum_compare1 v arg.
-
-Definition vsum_eq1 (v arg : val) : imonad val :=
-  VBool <$> vsum_equal1 v arg.
-
-Definition vsum_neq1 (v arg : val) : imonad val :=
-  VBool_by negb <$> vsum_equal1 v arg.
-
-Definition vsum_lt2 (v arg : val) : imonad val :=
-  VBool_by compare_ltb <$> vsum_compare2 v arg.
-
-Definition vsum_le2 (v arg : val) : imonad val :=
-  VBool_by compare_leb <$> vsum_compare2 v arg.
-
-Definition vsum_gt2 (v arg : val) : imonad val :=
-  VBool_by compare_gtb <$> vsum_compare2 v arg.
-
-Definition vsum_ge2 (v arg : val) : imonad val :=
-  VBool_by compare_geb <$> vsum_compare2 v arg.
-
-Definition vsum_eq2 (v arg : val) : imonad val :=
-  VBool <$> vsum_equal2 v arg.
-
-Definition vsum_neq2 (v arg : val) : imonad val :=
-  VBool_by negb <$> vsum_equal2 v arg.
-
-(** Tuple *)
-
-Definition vtuple_eq (t : tuple) (arg : val) : imonad val :=
-  VBool <$> vtuple_equal t arg.
-
-Definition vtuple_neq (t : tuple) (arg : val) : imonad val :=
-  VBool_by negb <$> vtuple_equal t arg.
-
-(** Record *)
-
-Definition vrecord_eq (r : record) (arg : val) : imonad val :=
-  VBool <$> vrecord_equal r arg.
-
-Definition vrecord_neq (r : record) (arg : val) : imonad val :=
-  VBool_by negb <$> vrecord_equal r arg.
-
-(** Variant *)
-
-Definition vvariant_eq (tag : tag) (v arg : val) : imonad val :=
-  VBool <$> vvariant_equal tag v arg.
-
-Definition vvariant_neq (tag : tag) (v arg : val) : imonad val :=
-  VBool_by negb <$> vvariant_equal tag v arg.
-
-(** Ref *)
-
-Definition vref_eq (l : loc) (arg : val) : imonad val :=
-  VBool_by2 loc_eqb l <$> unwrap_vref arg.
-
-Definition vref_neq (l : loc) (arg : val) : imonad val :=
-  VBool_by2 loc_neqb l <$> unwrap_vref arg.
-
-(** Exn *)
-
-Definition vexn_eq (tag : tag) (v arg : val) : imonad val :=
-  VBool <$> vexn_equal tag v arg.
-
-Definition vexn_neq (tag : tag) (v arg : val) : imonad val :=
-  VBool_by negb <$> vexn_equal tag v arg.
-
-(** Eff *)
-
-Definition veff_eq (tag : tag) (v arg : val) : imonad val :=
-  VBool <$> veff_equal tag v arg.
-
-Definition veff_neq (tag : tag) (v arg : val) : imonad val :=
-  VBool_by negb <$> veff_equal tag v arg.
-
-Definition dispatch_lt (v : val) : imonad (val -> imonad val) :=
-  match v with
-  | VTt => imonad_pure vunit_lt
-  | VInt z => imonad_pure (vint_lt z)
-  | VFloat q => imonad_pure (vfloat_lt q)
-  | VTrue => imonad_pure vbool_lt1
-  | VFalse => imonad_pure vbool_lt2
-  | VChar a => imonad_pure (vchar_lt a)
-  | VString s => imonad_pure (vstring_lt s)
-  | VPair v1 v2 => imonad_pure (vprod_lt v1 v2)
-  | VInl v' => imonad_pure (vsum_lt1 v')
-  | VInr v' => imonad_pure (vsum_lt2 v')
-  | _ => imonad_throw_error (Type_error "dispatch_lt")
-  end.
-
-Definition dispatch_le (v : val) : imonad (val -> imonad val) :=
-  match v with
-  | VTt => imonad_pure vunit_le
-  | VInt z => imonad_pure (vint_le z)
-  | VFloat q => imonad_pure (vfloat_le q)
-  | VTrue => imonad_pure vbool_le1
-  | VFalse => imonad_pure vbool_le2
-  | VChar a => imonad_pure (vchar_le a)
-  | VString s => imonad_pure (vstring_le s)
-  | VPair v1 v2 => imonad_pure (vprod_le v1 v2)
-  | VInl v' => imonad_pure (vsum_le1 v')
-  | VInr v' => imonad_pure (vsum_le2 v')
-  | _ => imonad_throw_error (Type_error "dispatch_le")
-  end.
-
-Definition dispatch_gt (v : val) : imonad (val -> imonad val) :=
-  match v with
-  | VTt => imonad_pure vunit_gt
-  | VInt z => imonad_pure (vint_gt z)
-  | VFloat q => imonad_pure (vfloat_gt q)
-  | VTrue => imonad_pure vbool_gt1
-  | VFalse => imonad_pure vbool_gt2
-  | VChar a => imonad_pure (vchar_gt a)
-  | VString s => imonad_pure (vstring_gt s)
-  | VPair v1 v2 => imonad_pure (vprod_gt v1 v2)
-  | VInl v' => imonad_pure (vsum_gt1 v')
-  | VInr v' => imonad_pure (vsum_gt2 v')
-  | _ => imonad_throw_error (Type_error "dispatch_gt")
-  end.
-
-Definition dispatch_ge (v : val) : imonad (val -> imonad val) :=
-  match v with
-  | VTt => imonad_pure vunit_ge
-  | VInt z => imonad_pure (vint_ge z)
-  | VFloat q => imonad_pure (vfloat_ge q)
-  | VTrue => imonad_pure vbool_ge1
-  | VFalse => imonad_pure vbool_ge2
-  | VChar a => imonad_pure (vchar_ge a)
-  | VString s => imonad_pure (vstring_ge s)
-  | VPair v1 v2 => imonad_pure (vprod_ge v1 v2)
-  | VInl v' => imonad_pure (vsum_ge1 v')
-  | VInr v' => imonad_pure (vsum_ge2 v')
-  | _ => imonad_throw_error (Type_error "dispatch_ge")
-  end.
-
-Definition dispatch_eq (v : val) : imonad (val -> imonad val) :=
-  match v with
-  | VTt => imonad_pure vunit_eq
-  | VInt z => imonad_pure (vint_eq z)
-  | VFloat q => imonad_pure (vfloat_eq q)
-  | VTrue => imonad_pure vbool_eq1
-  | VFalse => imonad_pure vbool_eq2
-  | VChar a => imonad_pure (vchar_eq a)
-  | VString s => imonad_pure (vstring_eq s)
-  | VPair v1 v2 => imonad_pure (vprod_eq v1 v2)
-  | VTuple t => imonad_pure (vtuple_eq t)
-  | VRecord r => imonad_pure (vrecord_eq r)
-  | VInl v' => imonad_pure (vsum_eq1 v')
-  | VInr v' => imonad_pure (vsum_eq2 v')
-  | VVariant tag v' => imonad_pure (vvariant_eq tag v')
-  | VRef l => imonad_pure (vref_eq l)
-  | VExn tag v' => imonad_pure (vexn_eq tag v')
-  | VEff tag v' => imonad_pure (veff_eq tag v')
-  | _ => imonad_throw_error (Type_error "dispatch_eq")
-  end.
-
-Definition dispatch_neq (v : val) : imonad (val -> imonad val) :=
-  match v with
-  | VTt => imonad_pure vunit_neq
-  | VInt z => imonad_pure (vint_neq z)
-  | VFloat q => imonad_pure (vfloat_neq q)
-  | VTrue => imonad_pure vbool_neq1
-  | VFalse => imonad_pure vbool_neq2
-  | VChar a => imonad_pure (vchar_neq a)
-  | VString s => imonad_pure (vstring_neq s)
-  | VPair v1 v2 => imonad_pure (vprod_neq v1 v2)
-  | VTuple t => imonad_pure (vtuple_neq t)
-  | VRecord r => imonad_pure (vrecord_neq r)
-  | VInl v' => imonad_pure (vsum_neq1 v')
-  | VInr v' => imonad_pure (vsum_neq2 v')
-  | VVariant tag v' => imonad_pure (vvariant_neq tag v')
-  | VRef l => imonad_pure (vref_neq l)
-  | VExn tag v' => imonad_pure (vexn_neq tag v')
-  | VEff tag v' => imonad_pure (veff_neq tag v')
-  | _ => imonad_throw_error (Type_error "dispatch_neq")
-  end.
-
-Definition dispatch_op2 (op : op2) : val -> imonad (val -> imonad val) :=
+Definition dispatch_op2 (op : op2) : val -> val -> imonad val :=
   match op with
   | Op2Add => dispatch_add
   | Op2Sub => dispatch_sub
